src/SDK/Serialize/HeaderV1.dfy
@@ -29,43 +29,38 @@ module HeaderV1 {
   | h.HeaderBodyV1?
   witness *
 
-  const VERSION_1: seq<uint8> := [0x01];
-  type Version = s: seq<uint8>
-  | s == VERSION_1
-  witness VERSION_1
-
   const RESERVED_BYTES: seq<uint8> := [0x00, 0x00, 0x00, 0x00];
   type ReservedBytes = s: seq<uint8>
   | s == RESERVED_BYTES
   witness RESERVED_BYTES
 
-  function method WriteHeaderBodyV1(
+  function method WriteV1HeaderBody(
     body: V1HeaderBody
-  ):
-    (ret: seq<uint8>)
+  )
+    :(ret: seq<uint8>)
   {
 
     var suiteId := GetAlgorithmSuiteId(body.esdkSuiteId);
     var suite := Client.SpecificationClient().GetSuite(suiteId);
 
-    WriteV1Version(VERSION_1)
+    Header.WriteVersion(Header.VERSION_1)
     + WriteV1MessageType(body.messageType)
-    + WriteESDKSuiteId(body.esdkSuiteId)
-    + WriteMessageId(body.messageId)
+    + Header.WriteESDKSuiteId(body.esdkSuiteId)
+    + Header.WriteMessageId(body.messageId)
     + WriteAADSection(body.encryptionContext)
     + WriteEncryptedDataKeys(body.encryptedDataKeys)
-    + WriteContentType(body.contentType)
+    + Header.WriteContentType(body.contentType)
     + WriteV1ReservedBytes(RESERVED_BYTES)
     + WriteV1HeaderIvLength(suite.encrypt.ivLength)
     + UInt32ToSeq(body.frameLength)
   }
 
-  function method ReadHeaderBodyV1(
+  function method ReadV1HeaderBody(
     bytes: ReadableBytes
   )
     :(res: ReadCorrect<V1HeaderBody>)
     ensures
-      || CorrectlyRead(bytes, res, WriteHeaderBodyV1)
+      || CorrectlyRead(bytes, res, WriteV1HeaderBody)
       // This is to handle the edge case in empty AAD see: `ReadAADSection`
       || (
         var headerBytesToAADStart := 20; 
@@ -74,27 +69,29 @@ module HeaderV1 {
         && aadStartPosition+4 < |bytes.data|
         && bytes.data[aadStartPosition..aadStartPosition+4] == [0,2,0,0]
         ==>
-          && CorrectlyRead(bytes, res, WriteExpandedAADSectionHeaderBodyV1))
+          && CorrectlyRead(bytes, res, WriteV1ExpandedAADSectionHeaderBody))
 
   {
-    var version :- ReadV1Version(bytes);
+    var version :- Header.ReadVersion(bytes);
+    :- Need(version.thing == Header.VERSION_1, Error("Message version must be version 1."));
 
     var messageType :- ReadV1MessageType(version.tail);
 
-    var esdkSuiteId :- ReadESDKSuiteId(messageType.tail);
+    var esdkSuiteId :- Header.ReadESDKSuiteId(messageType.tail);
+    var suiteId := GetAlgorithmSuiteId(esdkSuiteId.thing);
+    var suite := Client.SpecificationClient().GetSuite(suiteId);
+    :- Need(suite.commitment.None?, Error("Algorithm suite must not support commitment."));
 
-    var messageId :- ReadMessageId(esdkSuiteId.tail);
+    var messageId :- Header.ReadMessageId(esdkSuiteId.tail);
 
     var encryptionContext :- EncryptionContext2.ReadAADSection(messageId.tail);
 
     var encryptedDataKeys :- EncryptedDataKeys.ReadEncryptedDataKeysSection(encryptionContext.tail);
 
-    var contentType :- ReadContentType(encryptedDataKeys.tail);
+    var contentType :- Header.ReadContentType(encryptedDataKeys.tail);
 
     var reservedBytes :- ReadV1ReservedBytes(contentType.tail);
 
-    var suiteId := GetAlgorithmSuiteId(esdkSuiteId.thing);
-    var suite := Client.SpecificationClient().GetSuite(suiteId);
     var headerIvLength :- ReadV1HeaderIvLength(
       reservedBytes.tail,
       suite
@@ -116,26 +113,6 @@ module HeaderV1 {
     Success(Data(body, frameLength.tail))
   }
 
-  function method WriteV1Version(
-    version: Version
-  ):
-    (ret: seq<uint8>)
-  {
-    version
-  }
-
-  function method ReadV1Version(
-    bytes: ReadableBytes
-  )
-    :(res: ReadCorrect<Version>)
-    ensures CorrectlyRead(bytes, res, WriteV1Version)
-  {
-    var Data(raw, tail) :- SerializeFunctions.Read(bytes, |VERSION_1|);
-    :- Need(raw == VERSION_1, Error("Incorrect message version."));
-    var version: Version := raw;
-    Success(Data(version, tail))
-  }
-
   function method WriteV1MessageType(
     messageType: Header.MessageType
   ):
@@ -153,61 +130,6 @@ module HeaderV1 {
     var Data(raw, tail) :- SerializeFunctions.Read(bytes, 1);
     var messageType :- Header.MessageType.Get(raw[0]).MapFailure(e => Error(e));
     Success(Data(messageType, tail))
-  }
-
-  function method WriteESDKSuiteId(
-    esdkSuiteId: ESDKAlgorithmSuiteId
-  ):
-    (ret: seq<uint8>)
-  {
-    UInt16ToSeq(esdkSuiteId)
-  }
-
-  function method ReadESDKSuiteId(
-    bytes: ReadableBytes
-  )
-    :(res: ReadCorrect<ESDKAlgorithmSuiteId>)
-    ensures CorrectlyRead(bytes, res, WriteESDKSuiteId)
-  {
-    var Data(esdkSuiteId, tail) :- ReadUInt16(bytes);
-    :- Need(esdkSuiteId in VALID_IDS, Error("Algorithm suite ID not supported."));
-    Success(Data(esdkSuiteId, tail))
-  }
-
-  function method WriteMessageId(
-    messageId: Header.MessageID
-  ):
-    (ret: seq<uint8>)
-  {
-    messageId
-  }
-
-  function method ReadMessageId(
-    bytes: ReadableBytes
-  )
-    :(res: ReadBinaryCorrect<Header.MessageID>)
-    ensures CorrectlyRead(bytes, res, WriteMessageId)
-  {
-    SerializeFunctions.Read(bytes, Header.MESSAGE_ID_LEN)
-  }
-
-  function method WriteContentType(
-    contentType: Header.ContentType
-  ):
-    (ret: seq<uint8>)
-  {
-    [contentType.Serialize()]
-  }
-
-  function method ReadContentType(
-    bytes: ReadableBytes
-  )
-    :(res: ReadCorrect<Header.ContentType>)
-    ensures CorrectlyRead(bytes, res, WriteContentType)
-  {
-    var Data(raw, tail) :- SerializeFunctions.Read(bytes, 1);
-    var contentType :- Header.ContentType.Get(raw[0]).MapFailure(e => Error(e));
-    Success(Data(contentType, tail))
   }
 
   function method WriteV1ReservedBytes(
@@ -232,8 +154,8 @@ module HeaderV1 {
 
   function method WriteV1HeaderIvLength(
     ivLength: uint8
-  ):
-    (ret: seq<uint8>)
+  )
+    :(ret: seq<uint8>)
   {
     [ivLength]
   }
@@ -254,22 +176,22 @@ module HeaderV1 {
   // because it is *only* used for correctness.
   // This represents the sub-optimal encoding of AAD
   // where empty AAD is encoded with an extra 2 bytes.
-  function WriteExpandedAADSectionHeaderBodyV1(
+  function WriteV1ExpandedAADSectionHeaderBody(
     body: V1HeaderBody
-  ):
-    (ret: seq<uint8>)
+  )
+    :(ret: seq<uint8>)
   {
 
     var suiteId := GetAlgorithmSuiteId(body.esdkSuiteId);
     var suite := Client.SpecificationClient().GetSuite(suiteId);
 
-    WriteV1Version(VERSION_1)
+    Header.WriteVersion(Header.VERSION_1)
     + WriteV1MessageType(body.messageType)
-    + WriteESDKSuiteId(body.esdkSuiteId)
-    + WriteMessageId(body.messageId)
+    + Header.WriteESDKSuiteId(body.esdkSuiteId)
+    + Header.WriteMessageId(body.messageId)
     + WriteExpandedAADSection(body.encryptionContext)
     + WriteEncryptedDataKeys(body.encryptedDataKeys)
-    + WriteContentType(body.contentType)
+    + Header.WriteContentType(body.contentType)
     + WriteV1ReservedBytes(RESERVED_BYTES)
     + WriteV1HeaderIvLength(suite.encrypt.ivLength)
     + UInt32ToSeq(body.frameLength)
