src/SDK/Serialize/HeaderV2.dfy
@@ -3,6 +3,7 @@
 
 include "../../../libraries/src/Collections/Sequences/Seq.dfy"
 include "../../Generated/AwsCryptographicMaterialProviders.dfy"
+include "../../AwsCryptographicMaterialProviders/Client.dfy"
 include "../../StandardLibrary/StandardLibrary.dfy"
 include "../../Util/UTF8.dfy"
 include "./SerializableTypes.dfy"
@@ -15,6 +16,7 @@ module HeaderV2 {
   import Aws.Crypto
   import Seq
   import Header
+  import MaterialProviders.Client
   import opened EncryptedDataKeys
   import opened EncryptionContext2
   import opened SerializableTypes
@@ -23,28 +25,93 @@ module HeaderV2 {
   import opened UTF8
   import opened SerializeFunctions
 
-  type V2Header = h: Header.Header
-  | h.body.HeaderBodyV2?
+  type V2HeaderBody = h: Header.HeaderBody
+  | h.HeaderBodyV2?
   witness *
 
-  const VERSION_2: seq<uint8> := [0x01];
-
-  function method WriteHeaderV2(
-    header: V2Header
-  ):
-    (ret: seq<uint8>)
+  function method WriteV2Header(
+    body: V2HeaderBody
+  )
+    :(ret: seq<uint8>)
   {
-    var canonicalEC := CanonicalEncryptionContext(header.body.encryptionContext);
 
-    VERSION_2
-    + UInt16ToSeq(header.body.esdkSuiteId)
-    + header.body.messageId
-    + WriteAADSection(canonicalEC)
-    + WriteEncryptedDataKeys(header.body.encryptedDataKeys)
-    + [header.body.contentType.Serialize()]
-    + UInt32ToSeq(header.body.frameLength)
-    + header.body.suiteData
+    Header.WriteVersion(Header.VERSION_2)
+    + Header.WriteESDKSuiteId(body.esdkSuiteId)
+    + Header.WriteMessageId(body.messageId)
+    + WriteAADSection(body.encryptionContext)
+    + WriteEncryptedDataKeys(body.encryptedDataKeys)
+    + Header.WriteContentType(body.contentType)
+    + UInt32ToSeq(body.frameLength)
+    + Write(body.suiteData)
   }
 
+  function method ReadV2HeaderBody(
+    bytes: ReadableBytes
+  )
+    :(res: ReadCorrect<V2HeaderBody>)
+    ensures
+      || CorrectlyRead(bytes, res, WriteV2Header)
+      // This is to handle the edge case in empty AAD see: `ReadAADSection`
+      || (
+        var headerBytesToAADStart := 1+2+16;
+        var aadStartPosition := bytes.start+headerBytesToAADStart;
+        && res.Success?
+        && aadStartPosition+4 < |bytes.data|
+        && bytes.data[aadStartPosition..aadStartPosition+4] == [0,2,0,0]
+        ==>
+          && CorrectlyRead(bytes, res, WriteV2ExpandedAADSectionHeader))
 
+  {
+    var version :- Header.ReadVersion(bytes);
+    :- Need(version.thing == Header.VERSION_2, Error("Message version must be version 1."));
+
+    var esdkSuiteId :- Header.ReadESDKSuiteId(version.tail);
+    var suiteId := GetAlgorithmSuiteId(esdkSuiteId.thing);
+    var suite := Client.SpecificationClient().GetSuite(suiteId);
+    :- Need(suite.commitment.HKDF?, Error("Algorithm suite must support commitment."));
+
+    var messageId :- Header.ReadMessageId(esdkSuiteId.tail);
+
+    var encryptionContext :- EncryptionContext2.ReadAADSection(messageId.tail);
+
+    var encryptedDataKeys :- EncryptedDataKeys.ReadEncryptedDataKeysSection(encryptionContext.tail);
+
+    var contentType :- Header.ReadContentType(encryptedDataKeys.tail);
+
+    var frameLength :- ReadUInt32(contentType.tail);
+
+    var suiteData :- Read(frameLength.tail, suite.commitment.outputKeyLength as nat);
+
+    var body:V2HeaderBody := Header.HeaderBodyV2(
+      esdkSuiteId := esdkSuiteId.thing,
+      messageId := messageId.thing,
+      encryptionContext := encryptionContext.thing,
+      encryptedDataKeys := encryptedDataKeys.thing,
+      contentType := contentType.thing,
+      frameLength := frameLength.thing,
+      suiteData := suiteData.thing
+    );
+
+    Success(Data(body, frameLength.tail))
+  }
+
+  // This is *not* a function method,
+  // because it is *only* used for correctness.
+  // This represents the sub-optimal encoding of AAD
+  // where empty AAD is encoded with an extra 2 bytes.
+  function WriteV2ExpandedAADSectionHeader(
+    body: V2HeaderBody
+  )
+    :(ret: seq<uint8>)
+  {
+
+    Header.WriteVersion(Header.VERSION_2)
+    + Header.WriteESDKSuiteId(body.esdkSuiteId)
+    + Header.WriteMessageId(body.messageId)
+    + WriteExpandedAADSection(body.encryptionContext)
+    + WriteEncryptedDataKeys(body.encryptedDataKeys)
+    + Header.WriteContentType(body.contentType)
+    + UInt32ToSeq(body.frameLength)
+    + Write(body.suiteData)
+  }
 }
